AVLtree.dfy
@@ -49,6 +49,28 @@ class AVLtree {
         }
     }
 
+    method findNode(node: AVLnode, queryNum: int) returns (found_node: AVLnode?)
+        requires node.valid()
+        ensures found_node != null ==> found_node in node.nodes
+        // Why is this not working?
+        // ensures found_node != null ==> found_node.key == queryNum
+        decreases node.nodes 
+    {
+        var temp: AVLnode? := node;
+        if temp != null
+        {
+            if (temp.left != null && queryNum < node.key) {
+                temp := findNode(temp.left, queryNum);
+            }
+            else if (temp.right != null && queryNum > node.key) {
+                temp := findNode(temp.right, queryNum);
+            }
+        }
+
+        return temp;
+    }
+
+
     // Task 1
     /*
     method leftRotate()
